src/FrameStack/LogRel.v
@@ -1,10 +1,7 @@
-(*Require Export SubstSemantics.*)
-Require Export Termination.
-Require Export Equalities.
-
+From CoreErlang.FrameStack Require Export Termination.
 Import ListNotations.
 
-(** Because of this, preorder is enough *)
+(** Because of this, reasoning about preorder relations is enough *)
 Goal forall T : Type, forall R : relation T, Reflexive R -> Transitive R ->
   let R' := fun x y => R x y /\ R y x in Reflexive R' /\ Symmetric R' /\ Transitive R'.
 Proof.
@@ -17,136 +14,48 @@ Proof.
     - eapply H0; eauto.
 Qed.
 
-
-Definition ProgRes_of (norm : (list ValueExpression + Exception)) : ProgResult := 
-match norm with
-| inr exc => ExcRes exc
-| inl vl => ValSeqRes vl
-end.
-
-(*
-Definition frame_rel (n : nat)
-                     (Nrel : forall m, m <= n -> (list ValueExpression + Exception) -> (list ValueExpression + Exception) -> Prop)
-                     (F1 F2 : FrameStack) : Prop :=
-  FSCLOSED F1 /\ FSCLOSED F2 /\
-  (forall m (Hmn : m <= n) (vl1 vl2 : (list ValueExpression + Exception)),
-    Nrel m Hmn vl1 vl2 ->
-    | F1, ProgRes_of vl1 | m ↓ -> | F2, ProgRes_of vl2 | ↓).
-*)
-
 Definition exc_rel (n : nat)
-                    (Vrel : forall m, m <= n -> ValueExpression -> ValueExpression -> Prop)
+                    (Vrel : forall m, m <= n -> Val -> Val -> Prop)
                     (e1 e2 : Exception) : Prop :=
 match e1, e2 with
   | (class1, reason1, details1), (class2, reason2, details2)  =>
     class1 = class2 /\
     (forall m (Hmn : m <= n),
-    Vrel m Hmn (reason1)  (reason2) /\
-    Vrel m Hmn (details1) (details2))
+    Vrel m Hmn reason1 reason2 /\
+    Vrel m Hmn details1 details2)
 end.
 
+(* Normal forms are exceptions and value sequences! This is why there
+   is two clauses. *)
 Definition frame_rel (n : nat)
-                     (Vrel : forall m, m <= n -> ValueExpression -> ValueExpression -> Prop)
+                     (Vrel : forall m, m <= n -> Val -> Val -> Prop)
                      (F1 F2 : FrameStack) : Prop :=
   FSCLOSED F1 /\ FSCLOSED F2 /\
-  (forall m (Hmn : m <= n) (vl1 vl2 : list ValueExpression),
+  (forall m (Hmn : m <= n) (vl1 vl2 : ValSeq),
     list_biforall (Vrel m Hmn) vl1 vl2 ->
-    | F1, ValSeqRes vl1 | m ↓ -> | F2, ValSeqRes vl2 | ↓)
+    | F1, RValSeq vl1 | m ↓ -> | F2, RValSeq vl2 | ↓)
   /\
   (forall m (Hmn : m <= n) (e1 e2 : Exception),
     exc_rel m (fun m' H => Vrel m' (Nat.le_trans _ _ _ H Hmn)) e1 e2 ->
-    | F1, ExcRes e1 | m ↓ -> | F2, ExcRes e2 | ↓).
-
-(*
-Definition exp_rel (n : nat)
-                   (Nrel : forall m, m <= n -> (list ValueExpression + Exception) -> (list ValueExpression + Exception) -> Prop)
-                   (p1 p2 : Expression)
-                 : Prop :=
-  EXPCLOSED p1 /\ EXPCLOSED p2 /\
-  forall m (Hmn : m <= n) F1 F2,
-     frame_rel m (fun m' H => Nrel m' (Nat.le_trans _ _ _ H Hmn)) F1 F2 ->
-     | F1, ExpRes p1 | m ↓ -> | F2, ExpRes p2 | ↓
-.
-*)
-
+    | F1, RExc e1 | m ↓ -> | F2, RExc e2 | ↓).
 
 Definition exp_rel (n : nat)
-                   (Vrel : forall m, m <= n -> ValueExpression -> ValueExpression -> Prop)
-                   (p1 p2 : Expression)
+                   (Vrel : forall m, m <= n -> Val -> Val -> Prop)
+                   (p1 p2 : Exp)
                  : Prop :=
   EXPCLOSED p1 /\ EXPCLOSED p2 /\
   forall m (Hmn : m <= n) F1 F2,
      frame_rel m (fun m' H => Vrel m' (Nat.le_trans _ _ _ H Hmn)) F1 F2 ->
-     | F1, ExpRes p1 | m ↓ -> | F2, ExpRes p2 | ↓
+     | F1, RExp p1 | m ↓ -> | F2, RExp p2 | ↓
 .
 
-(*
-Fixpoint Nrel_rec  (n : nat)
-                    (Nrel : forall m, m <= n -> (list ValueExpression + Exception) -> (list ValueExpression + Exception) -> Prop)
-                    (n1 n2 : (list ValueExpression + Exception)) : Prop :=
-  match n1, n2 with
-  | inl vl1,  inl vl2   => True
-  | inr (class1, reason1, details1), inr (class2, reason2, details2)  =>
-    class1 = class2 /\
-    Nrel_rec n Nrel (inl [reason1])  (inl [reason2]) /\
-    Nrel_rec n Nrel (inl [details1]) (inl [details2])
-  | _,  _ => False
-  end.
-  
-  
+Fixpoint Vrel_rec (n : nat)
+                  (Vrel : forall m, m < n -> Val -> Val -> Prop)
+                  (v1 v2 : Val) : Prop :=
   VALCLOSED v1 /\ VALCLOSED v2 /\
   match v1, v2 with
   | VNil, VNil => True
-  | VLit l, VLit l' => if Equalities.Literal_eqb l l' then True else False
-  | VCons hd tl, VCons hd' tl' => Vrel_rec n Vrel hd hd' /\ Vrel_rec n Vrel tl tl'
-  | VTuple l, VTuple l' =>
-    (fix go l l' :=
-      match l, l' with
-        | [], []        => True
-        | x::xs, y::ys  => Vrel_rec n Vrel x y /\ go xs ys
-        | _,  _         => False
-      end) l l'
-  | VMap l, VMap l' => True (*
-    (forall i, i < length l ->
-    Vrel_rec n Vrel Excrel (fst (nth i l (VNil, VNil))) (fst (nth i l' (VNil, VNil))) /\
-    Vrel_rec n Vrel Excrel (snd (nth i l (VNil, VNil))) (snd (nth i l' (VNil, VNil)))) *)
-  (* 
-  | EFun vl1 b1, EFun vl2 b2 =>
-    if length vl1 =? length vl2 then
-     forall m (Hmn : m < n), forall (vals1 vals2 : list Exp),
-       length vals1 = length vl1 -> length vals2 = length vl2 ->
-       list_biforall (Vrel m Hmn) vals1 vals2 
-     ->
-       exp_rel m (fun m' H => Vrel m' (Nat.le_lt_trans _ _ _ H Hmn)) 
-                 (b1.[list_subst (EFun vl1 b1 :: vals1) idsubst])
-                 (b2.[list_subst (EFun vl2 b2 :: vals2) idsubst])
-     else False
-  *)
-  
-  | VClos ext id vc e, VClos ext' id' vc' e' =>
-    vc = vc' /\
-    (forall m (Hmn : m < n),
-     forall (vl1 vl2 : list ValueExpression),
-     length vl1 = vc -> length vl2 = vc ->
-     Vrel m Hmn vl1 vl2 ->
-     exp_rel m (fun m' H => Vrel m' (Nat.le_lt_trans _ _ _ H Hmn))
-                (Excrel_rec m (fun m' H => Vrel m' (Nat.le_trans _ _ _ H Hmn)))
-                (e.[list_subst ((convert_to_closlist ext)++vl1) idsubst])
-                (e'.[list_subst ((convert_to_closlist ext')++vl2) idsubst])
-   )
-  | _, _ => False
-  end
-.
-*)
-
-
-Fixpoint Vrel_rec  (n : nat)
-                    (Vrel : forall m, m < n -> ValueExpression -> ValueExpression -> Prop)
-                    (v1 v2 : ValueExpression) : Prop :=
-  VALCLOSED v1 /\ VALCLOSED v2 /\
-  match v1, v2 with
-  | VNil, VNil => True
-  | VLit l, VLit l' => if Equalities.Literal_eqb l l' then True else False
+  | VLit l, VLit l' => if Lit_beq l l' then True else False
   | VCons hd tl, VCons hd' tl' => Vrel_rec n Vrel hd hd' /\ Vrel_rec n Vrel tl tl'
   | VTuple l, VTuple l' =>
     (fix go l l' :=
@@ -159,19 +68,17 @@ Fixpoint Vrel_rec  (n : nat)
     (fix go l l' :=
       match l, l' with
         | [], []        => True
-        | (x1,x2)::xs, (y1,y2)::ys  => Vrel_rec n Vrel x1 y1 /\ Vrel_rec n Vrel x2 y2 /\ go xs ys
+        | (x1,x2)::xs, (y1,y2)::ys  => Vrel_rec n Vrel x1 y1 /\
+                                       Vrel_rec n Vrel x2 y2 /\
+                                       go xs ys
         | _,  _         => False
-      end) l l'
-    (*
-    (forall i, i < length l ->
-    Vrel_rec n Vrel Excrel (fst (nth i l (VNil, VNil))) (fst (nth i l' (VNil, VNil))) /\
-    Vrel_rec n Vrel Excrel (snd (nth i l (VNil, VNil))) (snd (nth i l' (VNil, VNil)))) *)
-  
+      end) l l'  
   | VClos ext id vc e, VClos ext' id' vc' e' =>
     vc = vc' /\
     (forall m (Hmn : m < n),
-     forall (vl1 vl2 : list ValueExpression),
-     length vl1 = vc -> length vl2 = vc ->
+     forall (vl1 vl2 : list Val),
+     length vl1 = vc -> (* list_biforall restricts the length of vl2, thus
+                           this is sufficient*)
      list_biforall (Vrel m Hmn) vl1 vl2 ->
      exp_rel m (fun m' H => Vrel m' (Nat.le_lt_trans _ _ _ H Hmn))
                 (e.[list_subst ((convert_to_closlist ext)++vl1) idsubst])
@@ -181,10 +88,10 @@ Fixpoint Vrel_rec  (n : nat)
   end
 .
 
-Definition Vrel : nat -> ValueExpression -> ValueExpression -> Prop :=
+Definition Vrel : nat -> Val -> Val -> Prop :=
   Fix Wf_nat.lt_wf _ Vrel_rec.
 
-Definition Erel (n : nat) (e1 e2 : Expression) : Prop :=
+Definition Erel (n : nat) (e1 e2 : Exp) : Prop :=
   exp_rel n (fun m _ => Vrel m) e1 e2.
 
 Definition Frel (n : nat) (K1 K2 : FrameStack) : Prop :=
@@ -199,40 +106,91 @@ Definition Excrel (n: nat) (ex1 ex2 : Exception) : Prop :=
 (** ξ and η assigns closed expressions to vars in Γ 
   Basically this says, ξ and η are equivalent pointwise for Γ
 *)
+Section Val_ind_weakened.
 
-(*
+Variables (P : Val -> Prop)
+          (Q : list Val -> Prop)
+          (R : list (Val * Val) -> Prop).
+Hypotheses
+  (HV1 : P VNil)
+  (HV2 : forall l : Lit, P (VLit l))
+  (HV3 : forall hd : Val, P hd -> forall tl : Val, P tl -> P (VCons hd tl))
+  (HV4 : forall (l : list Val), Q l -> P (VTuple l))
+  (HV5 : forall (l : list (Val * Val)), R l -> P (VMap l))
+  (HV6 : forall n : Var, P (VVar n))
+  (HV7 : forall n : FunId, P (VFunId n))
+  (HV8 : forall (ext : list (nat * nat * Exp)) (id params : nat) (e : Exp),
+  P (VClos ext id params e))
+  (HQ1: Q [])
+  (HQ2: forall (v : Val), P v -> forall (vl : list Val), Q vl -> Q (v::vl))
+  (HR1: R [])
+  (HR2: forall (v1 : Val), P v1 -> forall (v2 : Val), P v2 -> 
+   forall (vl : list (Val * Val)), R vl -> R ((v1,v2)::vl)).
+
+Fixpoint Val_ind_weakened (v : Val) : P v :=
+  match v as x return P x with
+  | VNil => HV1
+  | VLit l => HV2 l
+  | VCons hd tl => HV3 hd (Val_ind_weakened hd) tl (Val_ind_weakened tl)
+  | VTuple l => HV4 l (list_ind Q HQ1 (fun e ls => HQ2 e (Val_ind_weakened e) ls) l)
+  | VMap l => HV5 l (list_ind R HR1 (fun '(e1,e2) ls => HR2 e1 (Val_ind_weakened e1) e2 (Val_ind_weakened e2) ls) l)
+  | VVar n => HV6 n
+  | VFunId n => HV7 n
+  | VClos ext id vl e => HV8 ext id vl e
+  end.
+
+End Val_ind_weakened.
+
 Lemma Vrel_rec_pointwise {n : nat} :
-  forall (f g : forall m : nat, (m < n)%nat -> Exp -> Exp -> Prop),
+  forall (f g : forall m : nat, (m < n)%nat -> Val -> Val -> Prop),
     (forall (m : nat) (p : (m < n)%nat), f m p = g m p) ->
     Vrel_rec n f = Vrel_rec n g.
 Proof.
   intros.
-  unfold Vrel_rec.
   extensionality v1.
   extensionality v2. generalize dependent v2.
-  induction v1; try destruct v2; intros; auto.
-  f_equal. f_equal.
-
-  cbn. break_match_goal. 2: auto.
-  
-  f_equal. f_equal.
-  extensionality m.
-  extensionality Hmn.
-  extensionality v1'.
-  extensionality v2'.
-  rewrite H.
-  extensionality l1. extensionality l2.
-  extensionality bif.
-  f_equal.
-  extensionality m'.
-  extensionality H0.
-  trivial.
-
-  do 2 f_equal.
-  rewrite IHv1_1, IHv1_2; auto.
+  induction v1 using Val_ind_weakened with
+    (Q := Forall (
+      fun v1 => forall v2 : Val, Vrel_rec n f v1 v2 = Vrel_rec n g v1 v2
+    ))
+    (R := Forall (
+      fun '(v11, v12) =>
+        (forall v2 : Val, Vrel_rec n f v11 v2 = Vrel_rec n g v11 v2)
+      /\
+        (forall v2 : Val, Vrel_rec n f v12 v2 = Vrel_rec n g v12 v2)
+    )); try destruct v2; unfold Vrel_rec; intros; try reflexivity.
+  * f_equal. f_equal. rewrite IHv1_1, IHv1_2; reflexivity.
+  * do 2 f_equal.
+    generalize dependent l0. induction l; destruct l0; try reflexivity; cbn.
+    destruct_foralls; unfold Vrel_rec in *; f_equal.
+    - now rewrite H2.
+    - clear H2. now apply IHl with (l0 := l0) in H3.
+  * do 2 f_equal.
+    generalize dependent l0. induction l; destruct l0; try reflexivity; cbn.
+    destruct a, p.
+    destruct_foralls; simpl. f_equal. 2: f_equal.
+    - fold Vrel_rec in *. now rewrite (proj1 H2).
+    - fold Vrel_rec in *. now rewrite (proj2 H2).
+    - clear H2. now apply IHl with (l0 := l0) in H3.
+  * repeat f_equal.
+    extensionality m.
+    extensionality Hmn.
+    extensionality v1'.
+    extensionality v2'.
+    rewrite H.
+    extensionality l1.
+    extensionality bif.
+    f_equal.
+    extensionality m'.
+    extensionality H0.
+    trivial.
+  * auto.
+  * auto.
+  * auto.
+  * auto.
 Qed.
 
-Lemma Vrel_Fix_eq : forall {n : nat} {v1 v2 : Exp},
+Lemma Vrel_Fix_eq : forall {n : nat} {v1 v2 : Val},
   Vrel n v1 v2
   = 
   Vrel_rec n (fun (m : nat) (_ : m < n) => Vrel m) v1 v2.
@@ -243,22 +201,39 @@ Proof.
   trivial.
 Qed.
 
-Definition inf := EApp (EFun [] (EApp (EFunId 0) [])) [].
+Definition inf :=
+  ELetRec
+    [(0, °EApp (`VFunId (0, 0)) [])]
+    (EApp (`VFunId (0, 0)) []).
 
 Theorem inf_diverges :
   forall n Fs, ~|Fs, inf| n↓.
 Proof.
-  unfold inf.
-  intros. intro. induction n using lt_wf_ind. inversion H; try inversion_is_value. subst.
-  inversion H5; subst.
-  clear H5 H. simpl in H3.
-  eapply H0. 2: exact H3. lia.
+  intros. intro. induction n using Wf_nat.lt_wf_ind.
+  inv H. 2: inv H1.
+  * simpl in *. inv H6. inv H4. inv H2. inv H5. 2: inv H.
+    cbn in H7.
+    unfold inf in H0. specialize (H0 (1 + k) ltac:(nia)).
+    apply H0. econstructor. reflexivity. cbn. assumption.
 Qed.
 
 Scheme le_dep_ind := Induction for le Sort Prop.
 
+Ltac forall_to_Forall :=
+  match goal with
+  | [H : forall i : nat, i < length _ -> ?P (nth i _ _) |- _] =>
+    apply indexed_to_forall in H
+  end.
+Ltac foralls_to_Foralls :=
+  repeat forall_to_Forall.
+
+Ltac fdestruct_scopes :=
+  destruct_scopes;
+  foralls_to_Foralls;
+  destruct_foralls.
+
 Lemma Vrel_downclosed :
-  forall {n m : nat} {Hmn : m <= n} {v1 v2 : Exp},
+  forall {n m : nat} {Hmn : m <= n} {v1 v2 : Val},
     Vrel n v1 v2 ->
     Vrel m v1 v2.
 Proof.
@@ -266,24 +241,48 @@ Proof.
     intros;
     eauto.
   generalize dependent v2.
-  induction v1; destruct v2; intros; intuition; try break_match_hyp; intros.
-  rewrite Vrel_Fix_eq.
-  rewrite Vrel_Fix_eq in H.
-  unfold Vrel_rec at 1.
-  unfold Vrel_rec at 1 in H. intuition.
-
-  try break_match_hyp; intros. 2: contradiction.
-  simpl.
-  epose proof (H2 m1 _ vals1 vals2 H1 H3 H4). apply H5; auto.
-
-  rewrite Vrel_Fix_eq.
-  rewrite Vrel_Fix_eq in H. destruct H as [cl1 [cl2 H]].
-  split. 2: split. 1-2: auto.
-  simpl. simpl in H. intros.
-  specialize (IHv1_1 v2_1). specialize (IHv1_2 v2_2).
-  do 2 rewrite Vrel_Fix_eq in IHv1_1. do 2 rewrite Vrel_Fix_eq in IHv1_2.
-  split. apply IHv1_1, H. apply IHv1_2, H.
-Unshelve. lia.
+  induction v1 using Val_ind_weakened with
+  (Q := Forall (
+    fun v1 => forall v2 : Val, Vrel (S m0) v1 v2 -> Vrel m v1 v2
+  ))
+  (R := Forall (
+    fun '(v11, v12) =>
+      (forall v2 : Val, Vrel (S m0) v11 v2 -> Vrel m v11 v2)
+    /\
+      (forall v2 : Val, Vrel (S m0) v12 v2 -> Vrel m v12 v2)
+  )); try destruct v2; intros; intuition; try break_match_hyp; intros.
+  * rewrite Vrel_Fix_eq.
+    rewrite Vrel_Fix_eq in H. destruct H as [cl1 [cl2 H]].
+    split. 2: split. 1-2: auto.
+    simpl. simpl in H. intros.
+    specialize (IHv1_1 v2_1). specialize (IHv1_2 v2_2).
+    do 2 rewrite Vrel_Fix_eq in IHv1_1. do 2 rewrite Vrel_Fix_eq in IHv1_2.
+    split. apply IHv1_1, H. apply IHv1_2, H.
+  * rewrite Vrel_Fix_eq.
+    rewrite Vrel_Fix_eq in H. simpl in *.
+    intuition.
+    generalize dependent l0. induction l; intros; auto.
+    - destruct_foralls; destruct l0; intuition; simpl in *.
+      + specialize (H4 v). do 2 rewrite Vrel_Fix_eq in H4. now apply H4.
+      + apply H2; auto.
+        fdestruct_scopes. constructor; now apply indexed_to_forall.
+        fdestruct_scopes. constructor; now apply indexed_to_forall.
+  * rewrite Vrel_Fix_eq.
+    rewrite Vrel_Fix_eq in H. simpl in *.
+    intuition.
+    generalize dependent l0. induction l; intros; auto.
+    - destruct_foralls; destruct l0; intuition; simpl in *.
+      destruct a, p. intuition.
+      + specialize (H2 v1). do 2 rewrite Vrel_Fix_eq in H2. now apply H2.
+      + specialize (H7 v2). do 2 rewrite Vrel_Fix_eq in H7. now apply H7.
+      + apply H1; auto;
+        destruct_scopes.
+        constructor; intros; [apply (H6 (S i) ltac:(slia))|apply (H12 (S i) ltac:(slia))].
+        constructor; intros; [apply (H9 (S i) ltac:(slia))|apply (H11 (S i) ltac:(slia))].
+  * rewrite Vrel_Fix_eq. rewrite Vrel_Fix_eq in H.
+    unfold Vrel_rec at 1.
+    unfold Vrel_rec at 1 in H. intuition.
+    apply H3; auto. nia.
 Qed.
 
 Lemma Erel_downclosed :
@@ -298,18 +297,17 @@ Proof.
   intros. eapply (H1 m0); eauto. lia.
 Qed.
 
-Lemma Vrel_closed : forall {n : nat} {v1 v2 : Exp},
+Lemma Vrel_closed : forall {n : nat} {v1 v2 : Val},
     Vrel n v1 v2 ->
     VALCLOSED v1 /\ VALCLOSED v2.
 Proof.
   intros. rewrite Vrel_Fix_eq in H.
-  Search "pointwise" "Vrel".
-  destruct v1, v2; destruct H as [Cl1 [Cl2 H]]; try inversion_is_value;
+  destruct v1, v2; destruct H as [Cl1 [Cl2 H]];
   split; try contradiction.
   all: auto.
 Qed.
 
-Lemma Vrel_closed_l : forall {n : nat} {v1 v2 : Exp},
+Lemma Vrel_closed_l : forall {n : nat} {v1 v2 : Val},
     Vrel n v1 v2 ->
     VALCLOSED v1.
 Proof.
@@ -320,7 +318,7 @@ Qed.
 
 Global Hint Resolve Vrel_closed_l : core.
 
-Lemma Vrel_closed_r : forall {n : nat} {v1 v2 : Exp},
+Lemma Vrel_closed_r : forall {n : nat} {v1 v2 : Val},
     Vrel n v1 v2 ->
     VALCLOSED v2.
 Proof.
@@ -361,7 +359,6 @@ Proof.
 Qed.
 
 Global Hint Resolve Erel_closed_r : core.
-*)
 
 (** closing substitutions *)
 Definition Grel (n : nat) (Γ : nat) (ξ₁ ξ₂ : Substitution) : Prop :=
@@ -372,7 +369,7 @@ Definition Grel (n : nat) (Γ : nat) (ξ₁ ξ₂ : Substitution) : Prop :=
     | _, _ => False
     end.
 
-(*
+
 Lemma Grel_downclosed_helper : forall vals1 vals2 m n,
   m <= n -> length vals1 = length vals2 ->
   list_biforall (Vrel n) vals1 vals2 ->
@@ -398,38 +395,22 @@ Proof.
   unfold Grel; intros. intuition.
   repeat break_match_goal; specialize (H2 x H1); try rewrite Heqs in H2; try rewrite Heqs0 in H2; [ intuition (eauto using Vrel_downclosed) | contradiction | contradiction ].
 Qed.
-*)
 
 
-Definition Vrel_open (Γ : nat) (v1 v2 : ValueExpression) :=
+
+Definition Vrel_open (Γ : nat) (v1 v2 : Val) :=
   forall n ξ₁ ξ₂,
   Grel n Γ ξ₁ ξ₂
 ->
   Vrel n (substVal ξ₁ v1) (substVal ξ₂ v2).
 
 
-Definition Erel_open (Γ : nat) (e1 e2 : Expression) :=
-  forall n ξ₁ ξ₂,
-  Grel n Γ ξ₁ ξ₂
-->
-  Erel n (subst ξ₁ e1) (subst ξ₂ e2).
-
-(*Future work*)
-(*
-Definition Vrel_open (Γ : nat) (e1 e2 : Exp) :=
-  forall n ξ₁ ξ₂,
-  Grel n Γ ξ₁ ξ₂
-->
-  Vrel n (subst ξ₁ e1) (subst ξ₂ e2).
-
 Definition Erel_open (Γ : nat) (e1 e2 : Exp) :=
   forall n ξ₁ ξ₂,
   Grel n Γ ξ₁ ξ₂
 ->
   Erel n (subst ξ₁ e1) (subst ξ₂ e2).
-*)
 
-(*
 Lemma Erel_open_closed : forall {Γ e1 e2},
     Erel_open Γ e1 e2 ->
     forall ξ, SUBSCOPE Γ ⊢ ξ ∷ 0 ->
@@ -442,14 +423,33 @@ Proof.
   intuition idtac. break_match_goal.
   (* rewrite Vrel_Fix_eq. unfold Vrel_rec at 1. *)
   specialize (H0 x H1) as P'. rewrite Heqs in P'. clear dependent ξ.
-  * rewrite Vrel_Fix_eq. unfold Vrel_rec at 1.
-    induction e; intros; try inversion_is_value; auto; try lia.
-    constructor; auto. constructor; auto.
-    break_match_goal; intros; try congruence; try inversion Hmn.
-    rewrite Nat.eqb_refl in Heqb; congruence.
-
-    split. 2: split. auto. auto. intros. inversion P'. subst.
-    split. eapply IHe1; auto. eapply IHe2; auto.
+  * clear H H1 x e1 e2 Γ. rewrite Vrel_Fix_eq. revert P'. revert v.
+    einduction v using Val_ind_weakened with
+      (Q := Forall (
+        fun v => VALCLOSED v -> Vrel_rec 0 (fun (m : nat) (_ : m < 0) => Vrel m) v v
+      ))
+      (R := Forall (
+        fun '(v1, v2) =>
+         (VALCLOSED v1 -> Vrel_rec 0 (fun (m : nat) (_ : m < 0) => Vrel m) v1 v1) /\
+         (VALCLOSED v2 -> Vrel_rec 0 (fun (m : nat) (_ : m < 0) => Vrel m) v2 v2)
+      )); intros; auto.
+    all: split;[auto|split;auto].
+    - now rewrite Lit_eqb_refl.
+    - destruct_scopes. split. now eapply IHv0_1. now eapply IHv0_2.
+    - induction l; auto.
+      fdestruct_scopes. split.
+      + now apply H1.
+      + apply IHl; auto. constructor. now apply indexed_to_forall.
+    - induction l; auto.
+      fdestruct_scopes. destruct a. split. 2: split.
+      + apply H3. apply (H0 0). snia.
+      + apply H3. apply (H2 0). snia.
+      + apply IHl; auto. constructor.
+        intros. apply (H0 (S i)). snia.
+        intros. apply (H2 (S i)). snia.
+    - inv P'. nia.
+    - inv P'. nia.
+    - split; auto. intros. nia.
   * specialize (H0 x H1). rewrite Heqs in H0. lia.
 Qed.
 
